nola/examples/logic.v
@@ -126,11 +126,11 @@ Section iris.
   CoFixpoint ilist' N Φx : loc → ciProp Σ := ilist'_gen N Φx ilist'.
   Definition ilist N Φx : loc → ciProp Σ := ilist_gen N Φx ilist'.
 
-  (** ** Convert the predicate of [ilist] using [acsr] *)
+  (** ** Convert the predicate of [ilist] using [mod_acsr] *)
   Lemma ilist'_acsr `{!Deriv ih δ} {N Φx Ψx l} :
     □ (∀ δ' l', ⌜Deriv ih δ'⌝ → ⌜ih δ'⌝ →
-      acsr (fupd ∅ ∅) ⟦ Φx l' ⟧(δ') ⟦ Ψx l' ⟧(δ') ∧
-      acsr (fupd ∅ ∅) ⟦ Ψx l' ⟧(δ') ⟦ Φx l' ⟧(δ')) -∗
+      mod_acsr (fupd ∅ ∅) ⟦ Φx l' ⟧(δ') ⟦ Ψx l' ⟧(δ') ∧
+      mod_acsr (fupd ∅ ∅) ⟦ Ψx l' ⟧(δ') ⟦ Φx l' ⟧(δ')) -∗
       ⟦ ilist' N Φx l ⟧(δ) ∗-∗ ⟦ ilist' N Ψx l ⟧(δ).
   Proof.
     move: l. apply Deriv_ind=> ???. iIntros "#eqv".
@@ -140,26 +140,27 @@ Section iris.
       iApply inv'_acsr; iIntros "!>" (??[eqv ?]?).
     - iApply bi.and_elim_l. iApply "eqv"; [|done..]. iPureIntro.
       by apply Deriv_mono=> ?[??].
-    - iApply (wand_iff_acsr (M:=fupd _ _)). iModIntro. by iApply eqv.
+    - iApply (wand_iff_mod_acsr (M:=fupd _ _)). iModIntro. by iApply eqv.
     - iApply bi.and_elim_r. iApply "eqv"; [|done]. iPureIntro.
       by apply Deriv_mono=> ?[??].
-    - iApply (wand_iff_acsr (M:=fupd _ _)). iModIntro. rewrite wand_iff_comm.
-      by iApply eqv.
+    - iApply (wand_iff_mod_acsr (M:=fupd _ _)). iModIntro.
+      rewrite wand_iff_comm. by iApply eqv.
   Qed.
   Lemma ilist_acsr `{!Deriv ih δ} {N Φx Ψx l} :
     □ (∀ δ' l', ⌜Deriv ih δ'⌝ → ⌜ih δ'⌝ →
-      acsr (fupd ∅ ∅) ⟦ Φx l' ⟧(δ') ⟦ Ψx l' ⟧(δ') ∧
-      acsr (fupd ∅ ∅) ⟦ Ψx l' ⟧(δ') ⟦ Φx l' ⟧(δ')) -∗
+      mod_acsr (fupd ∅ ∅) ⟦ Φx l' ⟧(δ') ⟦ Ψx l' ⟧(δ') ∧
+      mod_acsr (fupd ∅ ∅) ⟦ Ψx l' ⟧(δ') ⟦ Φx l' ⟧(δ')) -∗
       ⟦ ilist N Φx l ⟧(δ) ∗-∗ ⟦ ilist N Ψx l ⟧(δ).
   Proof.
     iIntros "#eqv". rewrite /⟦ ⟧(δ) /=.
     iSplit; (iIntros "[ihd itl]"; iSplitL "ihd"; [iRevert "ihd"|iRevert "itl"]);
       iApply inv'_acsr; iIntros "!>" (????).
     - iApply bi.and_elim_l. by iApply "eqv".
-    - iApply (wand_iff_acsr (M:=fupd _ _)). iModIntro. by iApply ilist'_acsr.
-    - iApply bi.and_elim_r. by iApply "eqv".
-    - iApply (wand_iff_acsr (M:=fupd _ _)). iModIntro. rewrite wand_iff_comm.
+    - iApply (wand_iff_mod_acsr (M:=fupd _ _)). iModIntro.
       by iApply ilist'_acsr.
+    - iApply bi.and_elim_r. by iApply "eqv".
+    - iApply (wand_iff_mod_acsr (M:=fupd _ _)). iModIntro.
+      rewrite wand_iff_comm. by iApply ilist'_acsr.
   Qed.
 
   (** ** Termination of [iter] *)
