nola/iris/sinv_deriv.v
@@ -49,7 +49,7 @@ Section sinv_deriv.
     sinv_mod : iProp Σ → iProp Σ;
     sinv_mod_gen_upd :: GenUpd sinv_mod;
     sinv_jacsr_intp {δ P Q} :
-      ⟦ sinv_jacsr P Q ⟧(δ) ⊣⊢ acsr sinv_mod ⟦ P ⟧(δ) ⟦ Q ⟧(δ);
+      ⟦ sinv_jacsr P Q ⟧(δ) ⊣⊢ mod_acsr sinv_mod ⟦ P ⟧(δ) ⟦ Q ⟧(δ);
   }.
 
   Context `{!SinvDeriv}.
@@ -72,22 +72,22 @@ Section sinv_deriv.
   Lemma sinv_tok_sinv {P} : sinv_tok P ⊢ sinv δ P.
   Proof.
     rewrite sinv_unseal. iIntros "$ !>". iApply Deriv_to. iIntros (? _ _ _).
-    rewrite sinv_jacsr_intp. iApply (acsr_refl (M:=sinv_mod)).
+    rewrite sinv_jacsr_intp. iApply (mod_acsr_refl (M:=sinv_mod)).
   Qed.
 
   (** Allocate [sinv] *)
   Lemma sinv_alloc P : sinv_wsati δ ==∗ sinv δ P ∗ (⟦ P ⟧(δ) -∗ sinv_wsati δ).
   Proof. rewrite -sinv_tok_sinv. exact: sinv_tok_alloc. Qed.
 
-  (** Convert [sinv] with [acsr] *)
+  (** Convert [sinv] with [mod_acsr] *)
   Lemma sinv_acsr {P Q} :
     □ (∀ δ', ⌜Deriv ih δ'⌝ → ⌜ih δ'⌝ → ⌜dinto δ δ'⌝ →
-      acsr sinv_mod ⟦ P ⟧(δ') ⟦ Q ⟧(δ')) -∗
+      mod_acsr sinv_mod ⟦ P ⟧(δ') ⟦ Q ⟧(δ')) -∗
       sinv δ P -∗ sinv δ Q.
   Proof.
     rewrite sinv_unseal. iIntros "#PQP [%R[#RPR $]] !>". iApply Deriv_to.
     iIntros (??? to). rewrite sinv_jacsr_intp.
-    iApply (acsr_trans (M:=sinv_mod)). { by rewrite to sinv_jacsr_intp. }
+    iApply (mod_acsr_trans (M:=sinv_mod)). { by rewrite to sinv_jacsr_intp. }
     by iApply "PQP".
   Qed.
 
@@ -95,8 +95,8 @@ Section sinv_deriv.
   Local Lemma sinv_sep' {PQ P Q} :
     (∀ δ', ⟦ PQ ⟧(δ') ≡ (⟦ P ⟧(δ') ∗ ⟦ Q ⟧(δ'))%I) → sinv δ PQ ⊢ sinv δ P.
   Proof.
-    move=> eq. iApply sinv_acsr. iIntros "!>" (????). unfold acsr. rewrite eq.
-    iApply (acsr_sep_l (M:=sinv_mod)).
+    move=> eq. iApply sinv_acsr. iIntros "!>" (????). rewrite /mod_acsr eq.
+    iApply (mod_acsr_sep_l (M:=sinv_mod)).
   Qed.
   Lemma sinv_sep {PQ P Q} : (∀ δ', ⟦ PQ ⟧(δ') ≡ (⟦ P ⟧(δ') ∗ ⟦ Q ⟧(δ'))%I) →
     sinv δ PQ ⊢ sinv δ P ∗ sinv δ Q.
